messageInvariantPrototypes/toylock/distributedMonotonic/applicationProof.dfy
@@ -1,0 +1,72 @@
+include "messageInvariants.dfy"
+include "ownershipInvariants.dfy"
+
+module ToylockProof {
+  import opened Types
+  import opened UtilitiesLibrary
+  import opened DistributedSystem
+  import opened Obligations
+  import opened MessageInvariants
+  import opened OwnershipInvariants
+  
+  ghost predicate ApplicationInv(c: Constants, v: Variables)
+    requires v.WF(c)
+  {
+    true
+  }
+
+  ghost predicate Inv(c: Constants, v: Variables)
+  {
+    && MessageInv(c, v)
+    && OwnershipInv(c, v)
+    && ApplicationInv(c, v)
+    && Safety(c, v)
+  }
+
+  lemma InvImpliesSafety(c: Constants, v: Variables)
+    requires Inv(c, v)
+    ensures Safety(c, v)
+  {}
+
+  lemma InitImpliesInv(c: Constants, v: Variables)
+    requires Init(c, v)
+    ensures Inv(c, v)
+  {
+    InitImpliesMessageInv(c, v);
+  }
+
+  lemma InvInductive(c: Constants, v: Variables, v': Variables)
+    requires Inv(c, v)
+    requires Next(c, v, v')
+    ensures Inv(c, v')
+  {
+    MessageInvInductive(c, v, v');
+    OwnershipInvInductive(c, v, v');
+    AtMostOwnerPerKeyImpliesSafety(c, v');
+  }
+
+/***************************************************************************************
+*                                 InvNext Proofs                                       *
+***************************************************************************************/
+
+lemma AtMostOwnerPerKeyImpliesSafety(c: Constants, v: Variables)
+  requires v.WF(c)
+  requires AtMostOwnerPerKey(c, v)
+  ensures Safety(c, v)
+{
+  forall idx1, idx2 | 
+    && c.ValidIdx(idx1) 
+    && c.ValidIdx(idx2) 
+    && HoldsLock(c, v, idx1)
+    && HoldsLock(c, v, idx2)
+  ensures
+     idx1 == idx2
+  {
+    // triggers
+    assert Host.HostOwnsUniqueKey(c.hosts[idx1], v.Last().hosts[idx1], 0);
+    assert Host.HostOwnsUniqueKey(c.hosts[idx1], v.Last().hosts[idx1], 0);
+  }
+}
+
+}
+
